# {{ book.discrete_mathematics.chapter3.3_4.title }}
<!-- toc -->

## Principle of Inclusion and Exclusion (PIE)
$$ U $$: universal set, $$ a_1 $$, $$ a_2 $$, ..., $$ a_n $$: 性質, $$ A_i $$ = { $$ x \in U $$ | $$ x $$ 滿足 $$ a_i $$ }, $$ N $$($$ a_i $$) = $$ |A_i| $$, $$ N $$($$ \bar{a_i} $$) = $$ |\bar{A_i}| $$  
$$ \Rightarrow N $$($$ \bar{a_i} \bar{a_j} $$) = $$ |\bar{A_i} \cap \bar{A_j}| $$ = $$ |U| $$ - [$$ N $$($$ a_i $$) + $$ N $$($$ a_j $$)] + $$ N $$($$ a_i \cap a_j $$)  
$$ \Rightarrow N $$($$ \bar{a_i} \bar{a_j} \bar{a_k} $$) = $$ |\bar{A_i} \cap \bar{A_j} \cap \bar{A_k}| $$ = $$ |U| $$ - [$$ N $$($$ a_i $$) + $$ N $$($$ a_j $$) + $$ N $$($$ a_k $$)] + [$$ N $$($$ a_i \cap a_j $$) + $$ N $$($$ a_i \cap a_k $$) + $$ N $$($$ a_j \cap a_k $$)] - $$ N $$($$ a_i a_j a_k $$)  
$$ \Rightarrow \quad \vdots $$  
$$ \Rightarrow N $$($$ \bar{a_1} \bar{a_2} $$ ... $$ \bar{a_k} $$) = $$ \color{red}{|U|} $$ - $$ \color{orange}{\displaystyle\sum_{i=1}^n N(a_i)} $$ + $$ \color{green}{\displaystyle\sum_{1 \le i < j \le n} N(a_i a_j)} $$ - $$ \color{blue}{\displaystyle\sum_{1 \le i < j < k \le n} N(a_i a_j a_k)} $$ + ... + $$ \color{purple}{(-1)^n N(a_1 a_2 ... a_n)} $$  
= $$ \color{red}{S_0} $$ - $$ \color{orange}{S_1} $$ + $$ \color{green}{S_2} $$ - $$ \color{blue}{S_3} $$ + ... + $$ \color{purple}{(-1)^n S_n} $$, 其中 $$ S_r $$ 含 $$ \dbinom{n}{r} $$ 項之和
> **排容原理**即**文氏圖**，只看 **$$ U $$** 與**當下性質**

## Euler's Totient Function
$$ n \in Z^+ $$, $$ n $$ = $$ P^{e_1}_1 P^{e_2}_2 ... P^{e_k}_k $$ 為 $$ n $$ 的**質因數分解**，則 $$ \phi $$($$ n $$) = $$ n $$($$ 1 $$ - $$ \dfrac{1}{P_1} $$)($$ 1 $$ - $$ \dfrac{1}{P_2} $$)...($$ 1 $$ - $$ \dfrac{1}{P_k} $$)

###### proof: $$ k $$ = $$ 3 $$
$$ U $$ = { $$ 1 $$, $$ 2 $$, ..., $$ n $$ }, 令 $$ a_i $$ 表 $$ P_i $$ 之倍數, $$ i $$ = $$ 1 $$, $$ 2 $$, $$ 3 $$, $$ \phi $$($$ n $$) = $$ N $$($$ \bar{a_1} \bar{a_2} \bar{a_3} $$) = $$ S_0 $$ - $$ S_1 $$ + $$ S_2 $$ - $$ S_3 $$  
= $$ n $$ - [$$ \dfrac{n}{P_1} $$ + $$ \dfrac{n}{P_2} $$ + $$ \dfrac{n}{P_3} $$] + [$$ \dfrac{n}{P_1 P_2} $$ + $$ \dfrac{n}{P_1 P_3} $$ + $$ \dfrac{n}{P_2 P_3} $$] - $$ \dfrac{n}{P_1 P_2 P_3} $$  
= $$ n $$[$$ 1 $$ - ($$ \dfrac{1}{P_1} $$ + $$ \dfrac{1}{P_2} $$ + $$ \dfrac{1}{P_3} $$) + ($$ \dfrac{1}{P_1 P_2} $$ + $$ \dfrac{1}{P_1 P_3} $$ + $$ \dfrac{1}{P_2 P_3} $$) - $$ \dfrac{1}{P_1 P_2 P_3} $$]  
= $$ \dfrac{n}{P_1 P_2 P_3} $$[$$ P_1 P_2 P_3 $$ - ($$ P_1 P_2 $$ + $$ P_1 P_3 $$ + $$ P_2 P_3 $$) + ($$ P_1 $$ + $$ P_2 $$ + $$ P_3 $$) - $$ 1 $$]  
= $$ \dfrac{n}{P_1 P_2 P_3} $$($$ P_1 $$ - $$ 1 $$)($$ P_2 $$ - $$ 1 $$)($$ P_3 $$ - $$ 1 $$) = $$ n $$($$ \dfrac{P_1 - 1}{P_1} $$)($$ \dfrac{P_2 - 1}{P_2} $$)($$ \dfrac{P_3 - 1}{P_3} $$) = $$ n $$($$ 1 $$ - $$ \dfrac{1}{P_1} $$)($$ 1 $$ - $$ \dfrac{1}{P_2} $$)($$ 1 $$ - $$ \dfrac{1}{P_3} $$)

## Theorem of Onto Function Amount {#theorem-of-onto-function-amount}
$$ A $$, $$ B $$: sets, $$ |A| $$ = m, $$ |B| $$ = n, $$ m \ge n $$, 則 $$ f $$: $$ A \rightarrow B $$ **onto** 個數: $$ onto $$($$ m $$, $$ n $$) = $$ \displaystyle\sum_{i=0}^n $$($$ -1 $$)$$ ^i \dbinom{n}{i} $$($$ n $$ - $$ i $$)$$ ^m $$
> $$ m $$ 個相異球放入 $$ n $$ 個**相異**箱子，**不允許空箱**之方法數

###### proof:
$$ U $$ = { $$ f $$ | $$ f $$: $$ A \rightarrow B $$ } $$ \Rightarrow |U| $$ = $$ n^m $$, 令 $$ a_i $$ 表示 $$ U $$ 中函數滿足值域不含 $$ b_i $$ 之條件(**第 $$ i $$ 個箱子為空**), $$ i $$ = $$ 1 $$, ..., $$ n $$  
$$ \Rightarrow onto $$($$ m $$, $$ n $$) = $$ N $$($$ \bar{a_1} \bar{a_2} $$ ... $$ \bar{a_n} $$) = $$ S_0 $$ - $$ S_1 $$ + $$ S_2 $$ - $$ S_3 $$ + ... + ($$ -1 $$)$$ ^n S_n $$  
= $$ {\color{red}{\dbinom{n}{0}}} n^m $$ - $$ \dbinom{n}{1} $$($$ n $$ - $$ 1 $$)$$ ^m $$ + $$ \dbinom{n}{2} $$($$ n $$ - $$ 2 $$)$$ ^m $$ - $$ \dbinom{n}{3} $$($$ n $$ - $$ 3 $$)$$ ^m $$ + ... + ($$ -1 $$)$$ ^n \dbinom{n}{n} $$($$ n $$ - $$ n $$)$$ ^m $$  
= $$ \displaystyle\sum_{i=0}^n $$($$ -1 $$)$$ ^i \dbinom{n}{i} $$($$ n $$ - $$ i $$)$$ ^m $$
> ($$ -1 $$)$$ ^n \dbinom{n}{n} $$($$ n $$ - $$ n $$)$$ ^m $$ = $$ 0 $$

## Stirling Number of The Second Kind
$$ m $$, $$ n \in Z $$, $$ m \gt n \gt 1 $$  
$$ S $$($$ m $$, $$ n $$) = $$ \dfrac{onto(m, n)}{n!} $$ = $$ \dfrac{\displaystyle\sum_{i=0}^n (-1)^i \dbinom{n}{i} (n - i)^m}{n!} $$  
稱為**第二種 Stirling 數(Stirling number of the second kind)**
- 當 **$$ m $$ < $$ n $$** 時，$$ S $$($$ m $$, $$ n $$) = $$ 0 $$

> $$ m $$ 個相異球放入 $$ n $$ 個**相同**箱子，**不允許空箱**之方法數

$$ \rightarrow m $$ 個相異球放入 $$ n $$ 個**相同**箱子，**允許空箱**之方法數?
> $$ S $$($$ m $$, $$ n $$) + $$ S $$($$ m $$, $$ n $$ - $$ 1 $$) + ... + $$ S $$($$ m $$, $$ 1 $$)  
> - $$ S $$($$ m $$, $$ n $$): **$$ 0 $$ 個空箱**
> - $$ S $$($$ m $$, $$ n $$ - $$ 1 $$): **$$ 1 $$ 個空箱**  
> ...  
> - $$ S $$($$ m $$, $$ 1 $$): **$$ n $$ - $$ 1 $$ 個空箱**

### Theorem of S(m, n)
$$ m $$, $$ n \in N $$, $$ m \gt n \gt 2 $$, $$ S $$($$ m $$ + $$ 1 $$, $$ n $$) = $$ S $$($$ m $$, $$ n $$ - $$ 1 $$) + $$ n S $$($$ m $$, $$ n $$)

###### proof:
$$ S $$($$ m $$ + $$ 1 $$, $$ n $$): $$ m $$ + $$ 1 $$ 相異物分成恰 $$ n $$ 箱，固定一物 $$ A $$
1. $$ A $$ 所在的箱子**只有** $$ A $$: $$ S $$($$ m $$, $$ n $$ - $$ 1 $$)  
2. $$ A $$ 所在的箱子**不只有** $$ A $$: $$ n S $$($$ m $$, $$ n $$) $$ \rightarrow $$ 先放**除 $$ A $$ 之外的 $$ m $$ 個相異物入 $$ n $$ 箱**，再從其中**任一箱放入 $$ A $$**  

### Table of S(m, n)

| $$ \dfrac{n \rightarrow}{m \downarrow} $$ | 1 | 2 | 3 | 4 | 5 | 6 |
|:-:|:-:|:--:|:--:|:--:|:--:|:-:|
| 1 | 1 |    |    |    |    |   |
| 2 | 1 | 1  |    |    |    |   |
| 3 | 1 | 3  | 1  |    |    |   |
| 4 | 1 | 7  | 6  | 1  |    |   |
| 5 | 1 | 15 | 25 | 10 | 1  |   |
| 6 | 1 | 31 | 90 | 65 | 15 | 1 |

> $$ Example $$:  
> $$ \quad $$ $$ onto $$($$ 6 $$, $$ 3 $$) + $$ onto $$($$ 6 $$, $$ 3 $$) = ?  
> $$ solution $$:  
> $$ \quad $$ $$ 90 $$($$ 3! $$) + $$ 65 $$($$ 4! $$)